\documentclass[a4paper]{article}

\usepackage{fullpage} % Package to use full page
\usepackage{parskip} % Package to tweak paragraph skipping
\usepackage{tikz} % Package for drawing
\usepackage{amsmath}
\usepackage{hyperref}
\usepackage[utf8]{inputenc}
\usepackage{lmodern}
\usepackage[MeX]{polski}
\usepackage{listings}

\title{Binary Search}
\author{Ma≈Çgorzata Dymek}
\date{}

\begin{document}

\maketitle

\section{Average case complexiy}

\begin{equation*}
    A(n) = ave(X_n) = \sum_{k \geq 0}^{n}{p_{k_n} \cdot k}
    %\sum_{k=1}^{log_2n}{\frac{2^{k-1}}{n} \cdot k}
\end{equation*}

The probability of finding our element in the first step is $\frac{1}{n}$, as we search in n elements. However, in the second step it's $\frac{2}{n}$, because we're searching in  $\frac{n}{2}$ elements. Similarly for subsequent elements, so the probability of k'th element is $\frac{2^{k-1}}{n}$.

\begin{equation*}
    \sum_{k \geq 0}^{n}{p_{k_n} \cdot k} = \sum_{k=1}^{log_2n}{\frac{2^{k-1}}{n} \cdot k} =
    \frac{1}{n} \cdot 1 + \frac{2}{n} \cdot 2 + \frac{4}{n} \cdot 3 + \ldots +
    \frac{2^{log_2n -1}}{n} \cdot log_2n 
\end{equation*}

We can factor out $\frac{1}{n}$ and contiune:

\begin{equation*}
    1 \cdot 1 + 2 \cdot 2 + 4 \cdot 3 + \ldots + 2^{log_2n -1} \cdot log_2n = 
    2^{0} \cdot 1 + 2^{1} \cdot 2 + 2^{2} \cdot 3 + \ldots + 2^{log_2n -1} \cdot log_2
\end{equation*}

Let's take geometric series:

\begin{equation*}
    1 + x + x^2 + ... + x^m = \frac{x^{m+1} - 1}{x - 1} \cdot 1
\end{equation*}

And calculate the derivative of both sides of the equation:

\begin{equation*}
    0 + 1 + 2 \cdot x + 3 \cdot x^2 + ... + m \cdot x^{m-1} = 
    \frac{(m+1) \cdot x^m \cdot (x-1) - (x^{m+1} - 1)}{(x - 1)^2}
\end{equation*}

The result of the left side is similar to our sum. 

\begin{equation*}
    \frac{(m+1) \cdot x^m \cdot (x-1) - (x^{m+1} - 1)}{(x - 1)^2} = 
    \frac{(m+1) \cdot x^{m+1} - (m+1)x^m - x^{m+1} + 1}{(x - 1)^2} = 
    \frac{m \cdot x^{m+1}  - (m+1) \cdot x^m + 1}{(x-1)^2} 
\end{equation*}

Let's do a replacement: $x = 2$, $m = log_2n$.

\begin{align*}
    &\frac{log_2 \cdot 2^{log_2n+1}  - (log_2n+1) \cdot 2^{log_2n} + 1}{(2-1)^2} = 
    \frac{log_2n \cdot 2^{log_2n+1}  - (log_2n) \cdot 2^{log_2} - 2^{log_2n} + 1}{1} = \\&=
    log_2n \cdot 2^{log_2n} - 2^{log_2n} + 1 =
    2^{log_2n} \cdot (log_2n - 1) + 1 =
    n \cdot (log_2n - 1) + 1
\end{align*}


Now we can contiune with our sum.

\begin{equation*}
    \sum_{k=1}^{log_2n}{\frac{2^{k-1}}{n} \cdot k} =
    \frac{1}{n} \cdot (n \cdot (log_2n - 1) + 1) = 
    \frac{n \cdot (log_2n - 1) + 1}{n} = 
    log_2n - 1 + \frac{1}{n}
\end{equation*}

So $log_2n - 1 + \frac{1}{n}$ is the average case complexity, class $O(log_2n)$.


\section{Variancy of the average case complexity}

\begin{equation*}
var(X_n) = \sum_{k \geq 0}^{n}{(k - ave(X_n))^2 \cdot p_{k_n}}
\end{equation*}

We'll round our result to $log_2n$ to simplify calculations.

\begin{align*}
    &\sum_{k \geq 0}^{n}{(k - ave(X_n))^2 \cdot p_{k_n}} =
     \sum_{k = 1}^{log_2n}{(k - log_2n)^2 \cdot \frac{2^{k-1}}{n}} =
     \sum_{k = 1}^{log_2n}{(k^2 + (log_2n)^2 - 2 \cdot k \cdot log_2n) \cdot \frac{2^{k-1}}{n}} \\&=
     \frac{1}{n} (\sum_{k = 1}^{log_2n}{ k^2 \cdot 2^{k-1}} +
     \sum_{k = 1}^{log_2n}{(log_2n)^2 \cdot 2^{k-1}}
     - \sum_{k = 1}^{log_2n}{2^k \cdot k \cdot log_2n})
\end{align*}

\begin{equation*}
    \sum_{k = 1}^{log_2n}{ k^2 \cdot 2^{k-1}} = n \cdot (log_2n)^2 - 2 \cdot n \cdot log_2n + 3 \cdot n - 3
\end{equation*}

\begin{equation*}
    (log_2n)^2 \cdot \sum_{k = 1}^{log_2n}{2^{k-1}} = 
    n \cdot (log_2n)^2 - \frac{1}{2} \cdot (log_2n)^2
\end{equation*}

\begin{equation*}
    2 \cdot log_2n \cdot \sum_{k = 1}^{log_2n}{2^k \cdot k} =
    4 \cdot n \cdot (log_2n)^2 - 4 \cdot n \cdot log_2n + 4 \cdot log_2n
\end{equation*}

\begin{align*}
    &\sum_{k = 1}^{log_2n}{(k - log_2n)^2 \cdot \frac{2^{k-1}}{n}} =
     \frac{1}{n} \cdot (n \cdot (log_2n)^2 - 2 \cdot n \cdot log_2n + 3 \cdot n - 3 + n \cdot (log_2n)^2 - \frac{1}{2} \cdot (log_2n)^2 -\\&- 4 \cdot n \cdot (log_2n)^2 + 4 \cdot n \cdot log_2n - 4 \cdot log_2n ) = \frac{1}{n} ( -2 \cdot n \cdot (log_2n)^2 + 2 \cdot n \cdot log_2n - \frac{1}{2}\cdot (log_2n)^2 - n \cdot log_2n + 3 \cdot n - 3) =\\&=
     2 \cdot log_2n + 3 - ( 2 \cdot (log_2)^2 + \frac{1}{2n} (log_2n)^2 - \frac{4}{n} \cdot log_2n - \frac{3}{n} )
\end{align*}

So we received a result of class $O(log_2n)$.

\end{document}